Nat.lean
@@ -1,51 +1,63 @@
-inductive Nat' : Type
-  | zero : Nat'
-  | succ : Nat' → Nat'
+import Common.Meta
+import Mathlib.Logic.Equiv.Defs
 
-theorem Nat'.succ_inj : succ n = succ m → n = m :=
-  Eq.rec (motive := λ m _ => rec False (λ m _ => n = m) m) rfl
+private structure Sig where
+  Nat : Type
+  «Nat.zero» : Nat
+  «Nat.succ» : Nat → Nat
+  «Nat.rec₀» {motive : Nat → Prop} : motive «Nat.zero» → (∀ n, motive n → motive («Nat.succ» n)) → ∀ n, motive n
 
-theorem Nat'.succ_ne_zero : succ n ≠ zero :=
-  Eq.rec (motive := λ m _ => rec False (λ _ _ => True) m) trivial
+private structure Sig' (Imp : Sig) where
+  «Nat.rec» {motive : Imp.Nat → Sort u} : motive Imp.«Nat.zero» → (∀ n, motive n → motive (Imp.«Nat.succ» n)) → ∀ n, motive n
+  «Nat.rec_zero» {motive} zero succ : @«Nat.rec» motive zero succ Imp.«Nat.zero» = zero
+  «Nat.rec_succ» {motive} zero succ n : @«Nat.rec» motive zero succ (Imp.«Nat.succ» n) = succ n (@«Nat.rec» motive zero succ n)
 
-private def Nat'.rec' {motive : Nat' → Sort u} (zero : motive zero) (succ : ∀ n, motive n → motive n.succ) : ∀ n, motive n
-  | .zero => zero
-  | .succ n => succ n (rec' zero succ n)
+/-
+instance : Nonempty (Sig' Imp) := ⟨{
+  «Nat.rec» := λ {motive} zero succ n => Classical.choice <| @Sig.«Nat.rec₀» Imp (Nonempty <| motive ·) ⟨zero⟩ (⟨succ · <| Classical.choice ·⟩) n
+}⟩
+-/
 
-attribute [implementedBy Nat'.rec'] Nat'.rec
+instance : Nonempty (Sig' Imp) :=
+  let rec' {motive : _ → _} (zero : motive _) (succ : ∀ n, motive n → motive _) := 
+    @Sig.«Nat.rec₀» Imp (λ n => ∃ x, (∀ (h : n = Imp.«Nat.zero»), h ▸ x = zero) ∧ (∀ n' (h : n = Imp.«Nat.succ» n'), h ▸ x = succ n' sorry)) ⟨zero, λ _ => rfl, sorry⟩ (λ n ih => ⟨succ n (Classical.choose ih), sorry, sorry⟩)
+  ⟨{
+    «Nat.rec» := λ zero succ n => Classical.choose (rec' zero succ n)
+    «Nat.rec_zero» := λ zero succ => Classical.choose_spec (rec' zero succ Imp.«Nat.zero») |>.left rfl
+    «Nat.rec_succ» := λ zero succ n => by dsimp only []; show Classical.choose (rec' zero succ (Imp.«Nat.succ» n)) = succ n (Classical.choose (rec' zero succ n)); have := Classical.choose_spec (rec' zero succ (Imp.«Nat.succ» n)) |>.right n rfl; dsimp only [] at this; apply this.trans; clear this; sorry
+  }⟩
 
-def a : Nat' → Nat'
-  | .zero => .zero
-  | .succ i => .succ i
+private def Impl : Sig where
+  Nat := Nat
+  «Nat.zero» := .zero
+  «Nat.succ» := .succ
+  «Nat.rec₀» := @Nat.rec
 
-def b : Nat' → Nat'
-  | .zero => .zero
-  | .succ i => i
+private def Impl' : Sig' Impl where
+  «Nat.rec» := @Nat.rec
+  «Nat.rec_zero» _ _ := rfl
+  «Nat.rec_succ» _ _ _ := rfl
 
-def c : Nat' → Nat'
-  | .zero => .zero
-  | .succ i => c i
+private opaque Imp₁ : Sig := Impl
+private opaque Imp₁' : Sig' Imp₁ := unsafe opaque_def% Imp₁ ▸ Impl'
+def Nat₁ : Type := Imp₁.Nat
+def Nat₁.zero : Nat₁ := Imp₁.«Nat.zero»
+def Nat₁.succ : Nat₁ → Nat₁ := Imp₁.«Nat.succ»
+def Nat₁.rec {motive : Nat₁ → Sort u} : motive .zero → (∀ n, motive n → motive n.succ) → ∀ n, motive n := Imp₁'.«Nat.rec»
+@[simp] theorem Nat₁.rec_zero : ∀ zero succ, @Nat₁.rec motive zero succ .zero = zero := Imp₁'.«Nat.rec_zero»
+@[simp] theorem Nat₁.rec_succ : ∀ zero succ n, @Nat₁.rec motive zero succ (.succ n) = succ n (@Nat₁.rec motive zero succ n) := Imp₁'.«Nat.rec_succ»
 
-def d : Nat' → Nat'
-  | .zero => .zero
-  | .succ i => .succ (d i)
+private opaque Imp₂ : Sig := Impl
+private opaque Imp₂' : Sig' Imp₂ := unsafe opaque_def% Imp₂ ▸ Impl'
+def Nat₂ : Type := Imp₂.Nat
+def Nat₂.zero : Nat₂ := Imp₂.«Nat.zero»
+def Nat₂.succ : Nat₂ → Nat₂ := Imp₂.«Nat.succ»
+def Nat₂.rec {motive : Nat₂ → Sort u} : motive .zero → (∀ n, motive n → motive n.succ) → ∀ n, motive n := Imp₂'.«Nat.rec»
+@[simp] theorem Nat₂.rec_zero : ∀ zero succ, @Nat₂.rec motive zero succ .zero = zero := Imp₂'.«Nat.rec_zero»
+@[simp] theorem Nat₂.rec_succ : ∀ zero succ n, @Nat₂.rec motive zero succ (.succ n) = succ n (@Nat₂.rec motive zero succ n) := Imp₂'.«Nat.rec_succ»
 
-def a' : Nat' → Nat' :=
-  @Nat'.rec _
-    .zero
-    λ i _ => .succ i
-
-def b' : Nat' → Nat' :=
-  @Nat'.rec _
-    .zero
-    λ i _ => i
-
-def c' : Nat' → Nat' :=
-  @Nat'.rec _
-    .zero
-    λ _ c_i => c_i
-
-def d' : Nat' → Nat' :=
-  @Nat'.rec _
-    .zero
-    λ _ => .succ
+example : Nat₁ ≃ Nat₂ where
+  toFun := Nat₁.rec .zero λ _ => .succ
+  invFun := Nat₂.rec .zero λ _ => .succ
+  left_inv := Nat₁.rec (by simp) λ _ hn => by simp [hn]
+  right_inv := Nat₂.rec (by simp) λ _ hn => by simp [hn]
